ironfleet/ravana/Refinement.i.dfy
@@ -1,0 +1,99 @@
+include "Types.i.dfy"
+
+module Refinement_i {
+  import opened Types_i
+
+  predicate rstate_valid(rs: RState) {
+    true /* TODO */
+  }
+
+  predicate service_state_valid(ss: ServiceState) {
+    true /* TODO */
+  }
+
+  predicate refinement(rs: RState, ss: ServiceState)
+  {
+    rstate_valid(rs) &&
+    service_state_valid(ss) &&
+
+    //var master_node := rs_master_controller(rs);
+    var log := rs_log(rs);
+
+    var (fwdControllerState, fwdOutstandingCommands) :=
+          controller_state_looking_forward(log, rs.initControllerState);
+
+    var curOutstandingCommands := map_to_multiset(map
+          command_id : int | (
+            0 <= command_id < |fwdOutstandingCommands| &&
+            var command := master_node.buffered_commands[xid][command_id];
+            !(command_id in rs.servers[command.switch].received_command_ids)
+          ) ::
+            master_node.buffered_commands[xid][command_id]
+        );
+
+
+    /*
+    var curOutstandingCommands := set_to_multiset(set
+          xid : int , command_id : int | (
+            xid in master_node.buffered_commands &&
+            command_id in master_node.buffered_commands[xid] &&
+            var command := master_node.buffered_commands[xid][command_id];
+            !(command_id in rs.servers[command.switch].received_command_ids)
+          ) ::
+            ((xid, command_id), master_node.buffered_commands[xid][command_id])
+        );
+    */
+
+    ss.switchStates == (
+      map switch : EndPoint
+      | switch in rs_switches(rs)
+      :: rs.servers[switch].switchState
+    ) &&
+
+    ss.controllerState == fwdControllerState &&
+    ss.outstandingCommands == fwdOutstandingCommands &&
+
+    var outstandingEvents := set_to_multiset(set
+          switch : EndPoint, eid : int | (
+            switch in rs.servers &&
+            rs.servers[switch].NodeSwitch? &&
+            eid in rs.servers[switch].bufferedEvents
+          ) ::
+            ((switch, eid), rs.servers[switch].bufferedEvents[eid])
+        );
+
+    ss.outstandingEvents == outstandingEvents
+  }
+
+  function rs_logger_controller(rs: RState) : Node
+  requires rstate_valid(rs)
+  ensures Node.NodeLogger?
+  {
+    var ep :| ep in rs.servers && rs.servers[ep].NodeLogger?;
+    ep
+  }
+
+  function rs_log(rs: RState) : seq<LogEntry>
+  requires rstate_valid(rs)
+  {
+    rs_logger_controller(rs).log
+  }
+
+  function controller_state_looking_forward(
+      log: seq<LogEntry>,
+      controllerState: ControllerState) : (ControllerState, seq<SingleCommand>)
+  {
+    if |log| == 0 then
+      (controllerState, [])
+    else (
+      var elem := log[0];
+      if elem.LMProc then (
+        controller_state_looking_forward(log[1 .. ], controllerState)
+      ) else (
+        var cs', comms1 := controllerTransition(controllerState, elem.switch, elem.event);
+        var cs'', comms2 := controller_state_looking_forward(log[1 .. ], cs');
+        (cs'', comms1 + comms2)
+      )
+    )
+  }
+}
